Theorems for `toString` instances in `Pluto`.

src/M/Pluto/Language/AST.lean
@@ -7,12 +7,18 @@ import M.Pluto.Language.Constant
 namespace Pluto.Language
 
 
+open PlutusCore (ByteString Data)
+
+
 universe u
 
 
 structure Name where
   getName : String
 deriving Repr
+
+instance : ToString Name where
+  toString := Name.getName
 
 export Name (getName)
 
@@ -43,9 +49,61 @@ export Term (Var Lambda Apply Force Delay Constant Builtin Error Let IfThenElse)
 export BindingT (Binding)
 
 
+open BindingT Term
+
+mutual
+
+  def showBinding : BindingT ann → String
+    | Binding _ name term => toString name ++ " = " ++ showTerm term
+
+  def showBindings : List (BindingT ann) → String
+    | []      => ""
+    | [b]     => showBinding b
+    | b :: bs => showBinding b ++ "; " ++ showBindings bs
+
+  def showTerm' (term : Term ann) : String :=
+    let rec hasSpace : List Char → Bool
+              | []        => false
+              | ' ' :: _  => true
+              | _   :: xs => hasSpace xs
+    let s := showTerm term
+    if hasSpace s.toList
+      then "(" ++ s ++ ")"
+      else s
+
+  def intercalate' : List Name → String
+    | []      => ""
+    | [x]     => toString x
+    | x :: xs => toString x ++ " " ++ intercalate' xs
+
+  def showTerm : Term ann → String
+    | Var _ name                     => toString name
+    | Lambda _ names term            => "(\\" ++ intercalate' names ++ " -> " ++ showTerm term ++ ")"
+    | Apply _ term term'             => showTerm' term ++ " " ++ showTerm' term'
+    | Force _ term                   => "! " ++ showTerm' term
+    | Delay _ term                   => "# " ++ showTerm' term
+    | Constant _ cons                => toString cons
+    | Builtin _ builtin              => toString builtin
+    | Error _                        => "Error"
+    | Let _ []        term           => "let in " ++ showTerm term
+    | Let _ bindings term            => "let " ++ showBindings bindings ++ " in " ++ showTerm term
+    | IfThenElse _ term term' term'' => "if " ++ showTerm term ++ " then " ++ showTerm term' ++ " else " ++ showTerm term''
+ 
+end
+
+instance : ToString (BindingT ann) where
+  toString := showBinding
+
+instance : ToString (Term ann) where
+  toString := showTerm
+
+
 structure Program (ann : Type u) where
   unProgram : Term ann
 deriving Repr
+
+instance : ToString (Program ann) where
+  toString := toString ∘ Program.unProgram
 
 export Program (unProgram)
 
