src/M/Pluto.lean
@@ -1,6 +1,7 @@
 
 
 import M.Pluto.Language
+import M.Pluto.Proof
 
 
 namespace Pluto
