src/M/Pluto/Examples.lean
@@ -1,0 +1,94 @@
+
+
+import M.Pluto.Language
+
+
+namespace Pluto.Examples
+
+
+open Pluto.Language
+
+
+def echo : Term Unit :=
+  let x := Name.mk "x"
+  Lambda ()
+    [x]
+    $ Var () x
+
+#eval toString echo == "(\\x -> x)"
+
+
+def hello : Term Unit :=
+  let trace := Name.mk "trace"
+  let s := Name.mk "s"
+  let x := Name.mk "x"
+  let defaultGreeting := Name.mk "defaultGreeting"
+  let greet := Name.mk "greet"
+  let greeting := Name.mk "greeting"
+  let name := Name.mk "name"
+  let nameData := Name.mk "nameData"
+  Let ()
+    [
+      Binding () trace
+        $ Lambda () [s, x]
+        $ Apply ()
+          (
+            Apply ()
+              (
+                Force ()
+                  $ Builtin () Trace
+              )
+              $ Var () s
+          )
+          $ Var () x
+    , Binding () defaultGreeting
+        $ Constant () (T () "Hello")
+    , Binding () greet
+        $ Lambda () [greeting, name]
+        $ Apply ()
+          (
+            Apply ()
+              (Builtin () AppendString)
+              $ Apply ()
+                  (
+                    Apply ()
+                      (Builtin () AppendString)
+                      (Var () greeting)
+                  )
+                  $ Constant () (T () ", ")
+          )
+        $ Apply ()
+            (
+              Apply ()
+                (Var () trace)
+                (
+                  Apply ()
+                    (
+                      Apply ()
+                        (Builtin () AppendString)
+                        $ Constant () (T () "Name is: ")
+                    )
+                    $ Var () name
+                )
+            )
+            $ Var () name
+    ]
+    $ Lambda () [nameData]
+    $ Apply ()
+      (
+        Apply ()
+          (Var () greet)
+          (Var () defaultGreeting)
+      )
+      $ Apply ()
+        (Builtin () DecodeUtf8)
+        $
+          Apply ()
+            (Builtin () UnBData)
+            $ Var () nameData
+
+-- Test with `pluto run test.pluto 0x576f726c64`
+#eval toString hello == "let trace = (\\s x -> ((! Trace) s) x); defaultGreeting = \"Hello\"; greet = (\\greeting name -> (AppendString ((AppendString greeting) (\", \"))) ((trace ((AppendString (\"Name is: \")) name)) name)) in (\\nameData -> (greet defaultGreeting) (DecodeUtf8 (UnBData nameData)))"
+
+
+end Pluto.Examples
