src/M/Pluto/Proof/AST.lean
@@ -1,0 +1,142 @@
+
+
+import M.Pluto.Language.AST
+
+
+open Pluto.Language
+open PlutusCore (ByteString Data)
+
+
+private def test01 : Term Unit :=
+  Constant () $ I () 1
+
+example : toString test01 == "1" := rfl
+
+
+private def test02 : Term Unit :=
+  let x := Name.mk "x"
+  Lambda () [x]
+    $ Var () x
+
+theorem check02 : toString test02 == "(\\x -> x)" :=
+  by simp [toString, showTerm, test02]
+
+
+private def test03 : Term Unit :=
+  Let ()
+    [Binding () (Name.mk "x") $ Constant () $ I () 1]
+    $ Constant () $ I () 42
+
+example : toString test03 == "let x = 1 in 42" :=
+  by simp [toString, showBinding, showBindings, showTerm, test03]
+
+
+private def test04 : Term Unit :=
+  Let ()
+    [Binding () (Name.mk "id") test02]
+    $ Constant () $ I () 42
+  
+example : toString test04 == "let id = (\\x -> x) in 42" :=
+  by simp [toString, showTerm, test04, showBindings, showBinding, test02, check02]
+
+
+private def test05 : Term Unit :=
+  let f := Name.mk "f"
+  Let ()
+    [Binding () f test02]
+    $ Apply () (Var () f) (Constant () $ I () 1)
+  
+example : toString test05 == "let f = (\\x -> x) in f 1" :=
+  by simp [toString, showTerm, test05, showBindings, showBinding, test02, check02, intercalate', showTerm']
+
+
+private def test06 : Term Unit :=
+  let f := Name.mk "f"
+  let res := Name.mk "res"
+  Let ()
+    [Binding () f test02, Binding () res $ Delay () $ Apply () (Var () f) (Constant () $ I () 1)]
+    $ Var () res
+
+example : toString test06 == "let f = (\\x -> x); res = # (f 1) in res" :=
+  by simp [toString, showTerm, test06, showBindings, showBinding, test02, check02, intercalate', showTerm']
+
+
+private def test07 : Term Unit :=
+  let f := Name.mk "f"
+  let res := Name.mk "res"
+  Let ()
+    [Binding () f test02, Binding () res $ Delay () $ Apply () (Var () f) (Constant () $ I () 1)]
+    $ Force ()
+    $ Var () res
+
+example : toString test07 == "let f = (\\x -> x); res = # (f 1) in ! res" :=
+  by simp [toString, showTerm, test07, showBindings, showBinding, test02, check02, intercalate', showTerm']
+
+
+private def test08 : Term Unit :=
+  let iff := Name.mk "iff"
+  let cond := Name.mk "cond"
+  let x := Name.mk "x"
+  let y := Name.mk "y"
+  Let ()
+    [Binding () iff $ Lambda () [cond, x, y] $ IfThenElse () (Var () cond) (Var () x) (Var () y)]
+    $ Force ()
+    $ Apply ()
+      (
+        Apply ()
+          (Var () iff)
+          (Delay () $ Constant () $ I () 42)
+      )
+      (
+        Delay () $ Constant () $ I () 7
+      )
+
+example : toString test08 == "let iff = (\\cond x y -> if cond then x else y) in ! ((iff (# 42)) (# 7))" :=
+  by simp [toString, showTerm, test08, showBindings, showBinding, test02, check02, intercalate', showTerm']
+
+
+example : toString (Constant () $ B () true) == "True" := rfl
+
+
+example : toString (Constant () $ B () false) == "False" := rfl
+
+
+example : toString (Constant () $ I () 42) == "42" := rfl
+
+
+example : toString (Constant () $ I () (-2)) == "-2" := rfl
+
+
+example : toString (Constant () $ S () $ ByteString.mk $ ByteArray.mk #[0x41]) == "0x41" := rfl
+
+
+example : toString (Constant () $ T () "foobar") == "\"foobar\"" := rfl
+
+
+example : toString (Constant () $ U ()) == "()" := rfl
+
+
+example : toString (Constant () $ D () $ Data.I 42) == "data 42" := rfl
+
+
+example : toString (Constant () $ D () $ Data.B $ ByteString.mk $ ByteArray.mk #[0x41]) == "data 0x41" := rfl
+
+
+example : toString (Constant () $ D () $ Data.List [Data.I 1, Data.I 2, Data.I 3]) == "data [1,2,3]" :=
+  by simp [toString, showTerm, showData]
+
+
+example : toString (Constant () $ D () $ Data.List [Data.I 1, Data.B $ ByteString.mk $ ByteArray.mk #[0x41], Data.List [Data.I 42], Data.Map [(Data.B $ ByteString.mk $ ByteArray.mk #[0xfe], Data.I 7)]]) == "data [1,0x41,[42],{0xfe=7}]" :=
+  by simp [toString, showTerm, showData]
+
+
+example : toString (Constant () $ D () $ Data.Map [(Data.I 1, Data.B $ ByteString.mk $ ByteArray.mk #[0x42]), (Data.B $ ByteString.mk $ ByteArray.mk #[0xfe], Data.I 42),(Data.List [Data.I 1, Data.I 2], Data.List [Data.I 3, Data.I 4]),(Data.Map [(Data.I 1, Data.I 3)], Data.I 4)]) == "data {1=0x42,0xfe=42,[1,2]=[3,4],{1=3}=4}" :=
+  by simp [toString, showTerm, showData]
+
+
+example : toString (Constant () $ D () $ Data.Constr 0 [Data.I 1, Data.B $ ByteString.mk $ ByteArray.mk #[0x41]]) == "data sigma0.[1,0x41]" :=
+  by simp [toString, showTerm, showData]
+
+
+example : toString (Program.mk $ Lambda () [Name.mk "x"] (Constant () $ I () 3)) == "(\\x -> 3)" :=
+  by simp [toString, showTerm]
